Common/RTS_safe.thy
@@ -1,12 +1,13 @@
 (* File: RTS_safe.thy *)
 (* Author: Susannah Mansky, UIUC 2016 *)
-(* General model for Test Suites and Regression Test Selection algorithms *)
+(* General model for test suites and Regression Test Selection algorithms *)
 
 theory RTS_safe
 imports Main
 begin
 
-(* "Existence safe" RTS algorithm *)
+(* "Existence safe" RTS algorithm: if a test is deselected based on an output,
+ there is SOME matching under the changed program *)
 locale RTS_safe =
  fixes
   out :: "'prog \<Rightarrow> 'test \<Rightarrow> 'prog_out set" and
@@ -24,13 +25,15 @@ begin (* RTS_alg *)
 
 lemma equiv_out_refl: "equiv_out a a"
 using equiv_class_eq_iff equiv_out_equiv by fastforce
+
 lemma equiv_out_trans: "\<lbrakk> equiv_out a b; equiv_out b c \<rbrakk> \<Longrightarrow> equiv_out a c"
 using equiv_class_eq_iff equiv_out_equiv by fastforce
 
-(* HERE: make this description better *)
 (* Shows that it is safe to continue deselecting a test based on its output
  under a previous program, to an arbitrary number of program changes, as long as the
- test is continually deselected *)
+ test is continually deselected. This is useful because it means changed
+ programs don't need to generate new outputs for deselected tests to insure safety of
+ future deselections. *)
 lemma existence_safe_trans:
 assumes Pst_in: "Ps \<noteq> []" "set Ps \<subseteq> progs" "t \<in> tests" and
  o0: "o\<^sub>0 \<in> out (Ps!0) t" and
